proof/invariant-abstract/AARCH64/ArchBits_AI.thy
@@ -33,7 +33,7 @@ sublocale p_asid_table_current_vcpu_update:
   Arch_p_asid_table_update_eq "\<lambda>s. s\<lparr>arch_state := arm_current_vcpu_update f (arch_state s)\<rparr>"
   by (unfold_locales) auto
 
-sublocale p_asid_table_current_vcpu_update:
+sublocale p_asid_table_current_fpu_update:
   Arch_p_asid_table_update_eq "\<lambda>s. s\<lparr>arch_state := arm_current_fpu_owner_update f (arch_state s)\<rparr>"
   by (unfold_locales) auto
 
